theories/state.v
@@ -1,0 +1,96 @@
+Require Import syntax.
+Require Import util.
+Require Import vec.
+
+Definition value := option nat.
+
+Definition stack := nat -> value.
+Definition heap := { n & vec n value }.
+
+Definition empty_stack : stack := fun _ => None.
+Definition empty_heap : heap := existT _ O  tt.
+
+Definition newptr (h : heap) : heap * nat :=
+  match h with
+  | existT _ n l => (existT _ (S n) (append l None) , n)
+  end.
+
+Definition read (h : heap) (i : nat) : option value :=
+  match h with
+  | existT _ _ l => lookup l i
+  end.
+
+Definition hasptr (h : heap) (i : nat) : Prop :=
+  match h with
+  | existT _ n _ => i < n
+  end.
+
+Definition write (h : heap) (i : nat) (v : value) : heap :=
+  match h with
+  | existT _ n l =>
+      existT _ n (update l i v)
+  end.
+
+Definition state := ((stack * heap) + unit)%type.
+
+Definition good_state (s : stack) (h : heap) : state := inl (s , h).
+
+Notation "<{ s , h }>" := (good_state s h).
+
+Definition empty_state : state := <{ empty_stack, empty_heap }>.
+
+Definition mem_err : state := inr tt.
+
+Notation "'err'" := mem_err.
+
+Definition insert (x : nat) (v : value) (s : stack) : stack :=
+  fun y => if Nat.eq_dec x y then v else s y.
+
+Definition eval_expr (e : expr) (s : stack) : value :=
+  match e with
+  | Var x => s x
+  | Lit n => Some n
+  | Null => None
+  end.
+
+Definition isnat (s : stack) (e : expr) (n : nat) : Prop :=
+  match eval_expr e s with
+  | None => False
+  | Some n' => n = n'
+  end.
+
+Definition mapsto (h : heap) (i : nat) (v : value) : Prop :=
+  match read h i with
+  | None => False
+  | Some v' => v = v'
+  end.
+
+Definition is_true (v : value) : Prop :=
+  match v with
+  | Some n => n > 0
+  | None => False
+  end.
+
+Definition is_false (v : value) : Prop :=
+  match v with
+  | Some n => n = 0
+  | None => True
+  end.
+
+Lemma value_eq_dec (v1 v2 : value) : {v1 = v2} + {v1 <> v2}.
+Proof.
+  destruct v1 as [n1|]; destruct v2 as[n2|].
+  - destruct (Nat.eq_dec n1 n2).
+    + left. congruence.
+    + right. congruence.
+  - right. congruence.
+  - right. congruence.
+  - left. reflexivity.
+Qed.
+
+Lemma lookup_insert x v s : (insert x v s) x = v.
+Proof. 
+  intros. unfold insert. destruct (Nat.eq_dec x x); congruence.
+Qed.
+
+                       
